Fill in last current assumptions; get STLC and ICompilers closed under global context

src/named/Matches.v
@@ -11,7 +11,7 @@ Set Bullet Behavior "Strict Subproofs".
 From Ltac2 Require Import Ltac2.
 Set Default Proof Mode "Classic".
 From Utils Require Import Utils.
-From Named Require Import Exp.
+From Named Require Import Exp Rule.
 From Named Require Import Tactics.
 Require Import String.
 Import OptionMonad.
@@ -54,34 +54,19 @@ with args_match_unordered_fuel (fuel : nat)
        | _,_,_ => None
        end.
 
-
+(* The maximum depth of the expression is enough fuel for the matcher *)
 Fixpoint exp_depth (e: exp) : nat :=
   match e with
   | var _ => 0
   | con _ s => (foldl (fun n e => max (exp_depth e) n) 0 s).+1
   end.
-  
+
+(*
 Definition matches_unordered e pat :=
   do s <- matches_unordered_fuel (exp_depth pat) e pat;
      ! e == pat[/s/]; (* since we don't check merges, we check post-hoc *)
      ret s.
-
-(* This lemma is pretty much trivial, but it's the useful property.
-   A 'completeness' lemma is much harder, but also not as useful
-   for proofs of positive statements.
-*)
-Lemma matches_unordered_recognizes e pat s
-  : matches_unordered e pat = Some s ->
-    e = pat[/s/].
-Proof.
-  unfold matches_unordered.
-  ltac1:(case_match;[|inversion]).
-  ltac1:(case_match;[|inversion]).
-  symmetry in HeqH0.
-  intro seq; inversion seq; subst.
-  ltac1:(apply /eqP); assumption.
-Qed.
-
+ *)
 
 Fixpoint order_subst' s args : option subst :=
   match args with
@@ -92,6 +77,7 @@ Fixpoint order_subst' s args : option subst :=
        ret ((x,e)::s')
   end.
 
+(*
 Lemma order_subst'_vals s args s' p
   : all_fresh s ->
     order_subst' s args = Some s' ->
@@ -119,6 +105,7 @@ Proof.
       (*Lemma lookup_in
        *)
 Admitted.
+*)
 
 Definition order_subst s args :=
   (*guarantees that args is a permutation of (map fst s)
@@ -126,6 +113,7 @@ Definition order_subst s args :=
    *)
   if size s == size args then order_subst' s args else None.
 
+(*
 Lemma order_subst_vals s args s' p
   : all_fresh s ->
     order_subst s args = Some s' ->
@@ -138,30 +126,39 @@ Proof.
   ltac1:(case_match;[|inversion]).
   eauto using order_subst'_vals.
 Qed.
+*)
 
-
+(*
 Lemma matches_unordered_fuel_all_fresh e pat fuel s
   : matches_unordered_fuel fuel e pat = Some s ->
     all_fresh s.
 Proof.
   unfold matches_unordered.
+*)
 
+(*
 Lemma matches_unordered_all_fresh e pat s
   : matches_unordered e pat = Some s ->
     all_fresh s.
 Proof.
   unfold matches_unordered.
-  
+  *)
 
 (* Note that 'args' is critical to getting the order of the output subst correct.
    We assume of the input that FV(pat) is a permutation of args.
  *)
 Definition matches (e pat : exp) (args : list string) : option subst :=
-  do s <- matches_unordered e pat;
-    s' <- order_subst s args;
-ret s'.
+  do s <- matches_unordered_fuel (exp_depth pat) e pat;
+     s' <- order_subst s args;
+     (* this condition can fail because merge doesn't check for conflicts *)
+     !e == pat[/s'/];
+     ret s'.
 
-(* a lifting of the prior property*)
+
+(* This lemma is pretty much trivial, but it's the useful property.
+   A 'completeness' lemma is much harder, but also not as useful
+   for proofs of positive statements.
+*)
 Lemma matches_recognizes e pat args s
   : matches e pat args = Some s ->
     e = pat[/s/].
@@ -169,9 +166,61 @@ Proof.
   unfold matches.
   ltac1:(case_match;[|inversion]).
   ltac1:(case_match;[|inversion]).
-  symmetry in HeqH.
-  apply matches_unordered_recognizes in HeqH.
+  ltac1:(case_match;[|inversion]).
+  symmetry in HeqH1.
   intro seq; inversion seq; subst.
-Admitted  (*TODO: permutation lemmas.*).
+  ltac1:(apply /eqP); assumption.
+Qed.
+
+Lemma order_subst_args s args s'
+  : order_subst s args = Some s' ->
+    args = map fst s'.
+Proof.
+  unfold order_subst.
+  ltac1:(case_match;[|inversion]).
+  clear HeqH.
+  revert s'.
+  induction args; intro s'; simpl.
+  {
+    ltac1:(inversion); subst; reflexivity.
+  }
+  {
+    ltac1:(case_match;[|inversion]).
+    ltac1:(case_match;[|inversion]).
+    ltac1:(inversion).
+    simpl in *.
+    f_equal.
+    eauto.
+  }
+Qed.
+
+Lemma matches_args e pat args s
+  : matches e pat args = Some s ->
+    args = map fst s.
+Proof.
+  unfold matches.
+  ltac1:(case_match;[|inversion]).
+  ltac1:(case_match;[|inversion]).
+  ltac1:(case_match;[|inversion]).
+  ltac1:(inversion); subst.
+  eapply order_subst_args.
+  symmetry; eauto.
+Qed.
 
 
+
+Goal (matches (con "foo" [:: con "quox" [::]; con "bar" [:: con "baz"[::]]; var "b"])
+              (con "foo" [:: con "quox" [::]; var "b"; var "a"])
+              [:: "b"; "a"])%string.
+  unfold matches.
+  ltac1:(case_match).
+  simpl in HeqH.
+  vm_compute in HeqH.
+
+Notation "'{{e' e }}" := (e) (at level 0,e custom expr at level 100).
+Notation "'{{s' e }}" := (e) (at level 0,e custom srt at level 100).
+
+
+
+Goal (matches {{e #"foo" %"b" (#"bar" #"baz") #"quox"}}
+     {{e #"foo" %"a" %"b" #"quox"}} [:: "b"; "a"]).
