src/named/Exp.v
@@ -274,328 +274,7 @@ Qed.
 
 Instance substable_sort : Substable sort :=
   { subst_assoc := sort_subst_assoc }.
-    
-(*
 
-Lemma ws_lookup : forall d args (s : subst) n,
-    ws_subst args s -> n \in map fst s -> ws_exp args (named_list_lookup d s n).
-Proof.
-  intros d args.
-  elim; simpl; auto.
-  case.
-  intros n0 e0 s IH n.
-  simpl ws_subst.
-
-
-Theorem subst_preserves_ws
-  : forall e (s : subst) (csz : nat),
-    ws_exp (size s) e ->
-    ws_subst csz s ->
-    ws_exp csz (exp_subst s e).
-Proof using .
-  move => e s c wse.
-  move => wss.
-  pose (wss' := wss).
-  move: wss'.
-  rewrite /ws_subst.
-  move => elem_ws.
-  elim: e wse => //= => n.
-  - apply: ws_lookup => //=;
-    move: size_eq => /eqP -> //=.
-  - elim => //= x l' IHA IHB.
-    case /andP => xexp rexp.
-    case: IHB => IHB1 IHB2.
-    apply /andP. split; [auto|].
-    move: IHA -> => //=.
-Qed.
-
-
-Lemma shiftz (e : exp) : e^!0 = e.
-Proof using .
-  elim: e; simpl; auto.
-  intros; simpl.
-  unfold exp_shift.
-  simpl.
-  f_equal; auto.
-  elim: l H.
-  - by simpl; auto.
-  - simpl.
-    intros.
-    f_equal.
-    + destruct H0.
-      rewrite  -{2}H0.
-      by unfold exp_shift.
-    + apply: H.
-      destruct H0.
-      done.
-Qed.
-
-Lemma shift1_preserves_ws (e : exp) (n : nat)
-  : ws_exp n e -> ws_exp (n.+1) e^!1. 
-Proof using .
-  elim: e n.
-  - simpl; auto.      
-  - simpl.
-    intros until l.
-    elim: l.
-    + simpl; auto.
-    + simpl.
-      intros.
-      case: H0 => H00 H01.
-      move: H1; case /andP => wse H1.
-      apply /andP.
-      split; auto.
-Qed.
-
-
-Lemma map_ext {B C : Type} (f g : B -> C) (l : seq B)
-  : (forall e, f e = g e) -> map f l = map g l.
-Proof.
-  move => ext.
-  elim: l; try done.
-  move => e1 l' IH.
-  simpl.
-    by rewrite ext IH.
-Qed.
-
-Lemma map_ext' {B C : Type} (f g : B -> C) (v : seq B)
-  : forall (P : B -> bool),
-    (forall e, P e -> f e = g e) ->
-    List.fold_right (fun e => [eta andb (P e)]) true v ->
-    map f v = map g v.
-Proof.
-  move => P ext.
-  elim: v;[> done|].
-  move => e1 v' IH vfr.
-  simpl.
-  f_equal.
-  - rewrite ext => //.
-    move: vfr.
-    simpl.
-    by case /andP.
-  - apply: IH.
-    move: vfr; simpl; by case /andP.
-Qed.
-
-Lemma exp_var_map_map g fn (e : exp)
-  : exp_var_map g (exp_var_map (fun n => var (fn n)) e) = exp_var_map (fun n => g (fn n)) e.
-Proof.
-  elim: e => //.
-  - simpl. intros.
-    f_equal.
-    rewrite map_comp.
-    elim: l H => //.
-    simpl.
-    move => h t vfr.
-    case.
-    intros.
-    f_equal => //.
-    by apply: vfr.
-Qed.
-
-Lemma exp_var_map_ext f1 f2 (e : exp)
-  : (forall n, f1 n = f2 n) -> exp_var_map f1 e = exp_var_map f2 e.
-Proof.
-  move => ext.
-  elim: e; eauto.
-  move => s l H.
-  unfold exp_var_map.
-  fold exp_var_map.
-  f_equal.
-  elim: l H => //.
-  simpl.
-  intros.
-  case: H0 => -> IH.
-  f_equal.
-  auto.
-Qed.
-
-Lemma exp_var_map_ext' f1 f2 (e : exp) m
-  : ws_exp m e -> (forall n, n < m -> f1 n = f2 n) -> exp_var_map f1 e = exp_var_map f2 e.
-Proof.
-  move => wse ext.
-  elim: e wse ; eauto.
-  move => n l H wsv.
-  unfold exp_var_map.
-  fold exp_var_map.
-  f_equal.
-  simpl in wsv.
-  elim: l H wsv => //.
-  simpl.
-  intros.
-  case: H0 => IH1 IH.
-  move: wsv.
-  case /andP.
-  move /IH1 ->.
-  move /H.
-  intros.
-  f_equal.
-  auto.
-Qed.
-  
-Lemma shift1_decomp (e : exp) n : e^!(n.+1) = e^!n^!1.
-Proof.
-  elim: e n.
-  - simpl; auto.
-  - intros.
-    unfold exp_shift.
-    simpl.
-    f_equal.
-    rewrite -map_comp.
-    eapply map_ext.
-    intro e.
-    simpl.
-    rewrite exp_var_map_map.
-    f_equal.
-Qed.
-  
-Theorem shift_preserves_ws (e : exp) (n m : nat)
-  : ws_exp n e -> ws_exp (m + n) e^!m. 
-Proof.
-  elim: m e n.
-  - intros; rewrite shiftz.
-      by change (0 + n) with n.
-  - intros.
-    rewrite addSn.
-    rewrite shift1_decomp.
-    apply: shift1_preserves_ws.
-    auto.
-Qed.
-
-(* TODO: needed?
-Lemma lookup_in_shift_subst n' n m
-  : n' < n -> var_lookup (shift_subst n m) n' = var (n' + m).
-Proof.
-  Print shift_subst.
-  elim: n' n m.
-  - case => //.
-  - move => n IH.
-    case => //.
-    simpl.
-    intros.
-    change (n.+1 + m) with (n + m).+1.
-    rewrite addnC.
-    change (m + n).+1 with (m.+1 + n).
-    rewrite addnC.
-    eauto.
-Qed. 
-
-Theorem shift_subst_shift (e : exp) : forall n m, ws_exp n e ->  e [/shift_subst n m/] = e^!m.
-Proof.
-  elim: e.
-  - unfold exp_shift.
-    unfold exp_subst.
-    unfold exp_var_map.
-    intros; rewrite addnC;
-    eapply lookup_in_shift_subst.
-    auto.
-  - intros.
-    unfold exp_shift.
-    unfold exp_subst.
-    unfold exp_var_map.
-    f_equal.
-    pose H0' := H0.
-    simpl in H0'.
-    fold exp_var_map.
-    apply: map_ext'.
-    move => e ppf.
-    apply: exp_var_map_ext'.
-    exact ppf.
-    move => n1 n1lt.
-    rewrite addnC.
-    eapply lookup_in_shift_subst.
-    exact n1lt.
-    done.
-Qed.*)
-
-(* TODO: is this true? if so, prove
-Lemma id_subst {p} (e : exp p) : forall n m, e [/shift_subst n 0/] = e [/shift_subst m 0/].
-*)
-
-Lemma extract_var_shift n : var n = (var 0)^!n.
-Proof.
-  elim: n; simpl; auto.
-  intros.
-  rewrite shift1_decomp.
-  rewrite -H.
-  auto.
-Qed.
-
-
-(*TODO: how to do with levels?*)
-Fixpoint constr_shift n e :=
-  match e with
-  | var x => var x
-  | con m l => con (n + m) (map (constr_shift n) l)
-  end.
-
-
-Notation "e %! n" := (constr_shift n e) (at level 7).
-
-Notation "e ::%! n" := (map (constr_shift n) e) (at level 7).
-
-Lemma constr_shift0 e : e%!0 = e.
-Proof.
-  elim: e => //.
-  intros; simpl.
-  f_equal.
-  elim: l H => //.
-  simpl; intros.
-  case: H0 => H01 H02; f_equal; auto.
-Qed.
-
-Lemma map_constr_shift0 s : s::%!0 = s.
-  elim: s => //.
-  intros; simpl; f_equal; move: constr_shift0; auto.
-Qed.
-  
-Lemma constr_shift_shift e n m : e%!n %!m = e%!(n + m).
-Proof.
-  elim: e => //.
-  intros;
-    simpl;
-    f_equal.
-  - ring.
-  - elim: l H => //; simpl; intros.
-    rewrite -> H;
-      case: H0; intros.
-    f_equal; auto.
-    auto.
-Qed.
-
-Lemma map_constr_shift_shift l n m
-  : l ::%! n ::%! m = l::%!(n+m).
-Proof.
-  elim: l => //.
-  simpl.
-  move => a l ->.
-  f_equal; move: constr_shift_shift; auto.
-Qed.
-
-(* TODO: is this needed? if so, prove
-Lemma constr_shift_subst_comm e s n : e[/s/]%!n = e%!n[/s::%!n/].
-Proof.
-  elim: e s n.
-  - elim ;intro_to subst; case => //.
-  - intros; simpl;
-      unfold exp_subst;
-      unfold exp_var_map;
-      fold exp_var_map;
-      fold exp_subst.
-    f_equal.
-    fold exp_subst.
-    elim: l H => //.
-    simpl; intro_to and.
-    case; intros.
-    f_equal; eauto.
-Qed.
-*)
-*)
-
-Definition eq_pr {A B} eq_a eq_b (p1 p2 : A*B) : bool :=
-  let (a1,b1) := p1 in
-  let (a2,b2) := p2 in
-  (eq_a a1 a2) && (eq_b b1 b2).
 
 Fixpoint eq_exp e1 e2 {struct e1} : bool :=
   match e1, e2 with
@@ -605,53 +284,21 @@ Fixpoint eq_exp e1 e2 {struct e1} : bool :=
   | _,_ => false
   end.
 
-(*
-Lemma exp2_ind (P : exp -> exp -> Set)
-  : (forall n m, P (var n) (var m)) ->
-    (forall n c l, P (var n) (con c l)) ->
-    (forall n c l, P (con c l) (var n)) ->
-    (forall c1 c2, P (con c1 [::]) (con c2 [::])) ->
-    (forall c1 c2 a l, P (con c1 [::]) (con c2 (a::l))) ->
-    (forall c1 c2 a l, P (con c1 (a::l)) (con c2 [::])) ->
-    (forall c1 c2 a1 a2 l1 l2,
-        P a1 a2 ->
-        P (con c1 l1) (con c2 l2) ->
-        P (con c1 (a1::l1)) (con c2 (a2::l2))) ->
-    forall e1 e2, P e1 e2.
-Proof using .
-  intro_to exp.
-  elim.
-  - intro_to exp; case; auto.
-  - intro_to exp.
-    case; auto.
-    move => n0.
-    elim: l X.
-    + move => _; case; auto.
-    + move => a l IH.
-      simpl; case => pa fld.
-      case; auto.
-Qed.      
-
-(*TODO: case neq does not use the right name*)
-Tactic Notation "case_on_eqb" ident(a) ident(b) :=
-  let neq := fresh "neq" in
-  case neq: (a == b); constructor;
-  [f_equal; apply /eqP
-  | case => /eqP; rewrite neq].
-  
 
 Lemma eq_exp_refl : forall e, eq_exp e e.
 Proof.
   elim; simpl; auto.
   move => n.
-  suff: n == n.
-  move ->; simpl.
+  apply eqb_refl.
+  intro n.
   elim; simpl; auto.
+  rewrite eqb_refl; auto.
   intro_to and.
   case => eqaa fld.
   apply /andP.
   split; auto.
-  elim: n; simpl; auto.
+  apply /eqb_refl.
+  move: (H fld) => H'; break; break_goal; auto.
 Qed.
 
 Lemma all2_eq_exp_refl : forall l, all2 eq_exp l l.
@@ -660,55 +307,68 @@ Lemma all2_eq_exp_refl : forall l, all2 eq_exp l l.
   intros; apply /andP; split; auto.
 Qed.
 
-*)
 
 Lemma eq_expP : forall e1 e2, reflect (e1 = e2) (eq_exp e1 e2).
-Admitted.
-(*Proof.
-  elim.
-  - intro_to exp; case; simpl.
-    + move => n0.
-        by case_on_eqb n n0.
-    + constructor; by case.
-  - intro_to exp; case; simpl.
-    + constructor; by case.
-    + intros.
-      case neq: (n == n0); simpl.
-      * case alleq: (all2 eq_exp l l0).
-        --constructor.
-          f_equal.
-            by apply /eqP; rewrite neq.
-            elim: l X l0 alleq.
-          ++ simpl; move => _; case; by auto.
-          ++ simpl; move => a l IH.
-             case => refla fld.
-             case; try by auto.
-             move => a0 l0.
-             case /andP.
-             move /refla => -> all2l.
-             f_equal.
-             eauto.
-        -- constructor.
-           case => _.
-           elim: l X l0 alleq.
-           ++ simpl; move => _; case; by auto.
-          ++ simpl; move => a l IH.
-             case => refla fld.
-             case; try by auto.
-             move => a0 l0.
-             move /andP => oneof.
-             case => aeq leq.
-             apply oneof.
-             split.
-             rewrite aeq.
-             apply: eq_exp_refl.
-             rewrite leq.
-             apply: all2_eq_exp_refl.
-      * constructor.
-        case; move /eqP; by rewrite neq.
-Qed.*)        
-                
-
+  intro e1.
+  induction e1; intro e2; destruct e2; simpl; try by constructor.
+  {
+    destruct_reflect_bool.
+    f_equal; apply /eqP; symmetry; assumption.
+    case => /eqP.
+    change (?n == ?s) with (n=? s)%string.
+    rewrite - Heqb.
+    inversion.
+  }
+  {
+    destruct_reflect_andb_l; simpl;
+      [|constructor;
+        case; intros; subst;
+        rewrite eqb_refl in Heqb;
+        inversion Heqb ].
+    symmetry in Heqb.
+    move: Heqb =>/eqP ->.
+    suff: (reflect (l=l0) (all2 eq_exp l l0)).
+    {
+      move => lP; destruct_reflect_bool.
+      {
+        f_equal.
+        by apply /lP.
+      }
+      {
+        case.
+        move /lP; inversion.
+      }
+    }
+    {
+      clear n s.
+      revert l0 X.
+      induction l; intro l0; destruct l0; simpl; try by constructor.
+      intros; break.
+      destruct_reflect_andb_l.
+      symmetry in Heqb.
+      {
+        move: Heqb => /r Heqb; subst; simpl.
+        destruct_reflect_bool; [f_equal | inversion].
+        {
+          symmetry in Heqb.
+          move: Heqb => /IHl; auto.
+        }
+        {
+          subst.
+          rewrite all2_eq_exp_refl in Heqb.
+          inversion Heqb.
+        }
+      }
+      {
+        constructor.
+        inversion; subst.
+        rewrite eq_exp_refl in Heqb.
+        inversion Heqb.
+      }
+    }
+  }
+Qed.          
+     
 Definition exp_eqMixin := Equality.Mixin eq_expP.
 
 Canonical exp_eqType := @Equality.Pack exp exp_eqMixin.
@@ -719,85 +379,12 @@ Definition eq_sort (t1 t2 : sort) :=
   (n1 == n2) && (s1 == s2).
 
 Lemma eq_sortP s1 s2 : reflect (s1 = s2) (eq_sort s1 s2).
-Admitted.
+  destruct s1; destruct s2; simpl; solve_reflect_norec.
+Qed.
 
 Canonical sort_eqType := @Equality.Pack sort (Equality.Mixin eq_sortP).
+
 (*
-
-(* TODO: how to do for levels? any different?*)
-(* TODO: write a predlike version?/nonoption?*)
-Fixpoint constr_downshift n e : option exp :=
-  match e with
-  | var x => Some (var x)
-  | con m l =>
-    if n <= m
-    then Option.map (con (m - n)) (try_map (constr_downshift n) l)
-    else None
-  end.
-
-Lemma add_sub n n0 : n0 + n - n0 = n.
-Proof.
-  elim: n0 => //=.
-  rewrite sub_0_r.
-  by compute.
-Qed.
-  
-Lemma downshift_left_inverse e n : constr_downshift n e%!n = Some e.
-Proof.
-  elim: e n; [by simpl|].
-  intros; simpl.
-  rewrite leq_addr.
-  rewrite try_map_map_distribute.
-  change (Some (con n l)) with (omap (con n) (Some l)).
-  f_equal.
-  f_equal; by apply add_sub.
-  elim: l H => //=.
-  intros.
-  case: H0 => shifta shiftl.
-  rewrite shifta.
-  specialize (H shiftl).
-  rewrite H.
-  by compute.
-Qed.
-
-Lemma try_map_downshift_left_inverse l n : try_map (constr_downshift n) l::%!n = Some l.
-Proof.
-  elim: l => //=; intros.
-  rewrite downshift_left_inverse H.
-  by compute.
-Qed.
-
-Lemma add_inj_r n m1 m2 : n + m1 = n + m2 -> m1 = m2.
-Proof.
-  elim: n => //=.
-  eauto.
-Qed.
-  
-Lemma constr_shift_inj e1 e2 n : e1 %!n = e2 %!n -> e1 = e2.
-Proof.
-  elim: e1 e2; intro_to exp; case => //=.
-  move => n1 l0.
-  case.
-  move /add_inj_r -> => shift_eq.
-  f_equal.
-  move: shift_eq.
-  elim: l l0 H; intros until l0; case: l0 => //=.
-  intro_to and.
-  case => IH_a0 IHl.
-  case.
-  move /IH_a0 -> => shifteq.
-  f_equal.
-  eauto.
-Qed.
-
-Lemma seq_constr_shift_inj l1 l2 n : l1 ::%!n = l2 ::%!n -> l1 = l2.
-Proof.
-  elim: l1 l2; intros until l2; case: l2 => //=.
-  move => a0 l0.
-  case.
-  by move /constr_shift_inj -> => /H ->.
-Qed.
-
 
 Require Import String.
 Section Printing.
@@ -856,201 +443,6 @@ Section Printing.
 
 End Printing.
 
-
-Lemma
-  exp_subst_ind' (P : exp -> Prop) (Q : subst -> Prop)
-  : (forall n,  P (var n)) ->
-    (forall n s,  Q s -> P (con n s)) ->
-    Q [::] ->
-    (forall e s, P e -> Q s -> Q (e :: s)) ->
-    forall e, P e.
-Proof using .
-  intros.
-    elim: e; auto.
-    move=> n.
-    elim.
-    auto.
-    intros.
-    simpl in H4.
-    destruct H4.
-    apply H0.
-    apply H2; auto.
-    clear H3.
-    elim: l H5; auto.
-    intros.
-    destruct H5.
-    apply H2; auto.
-Qed.
-
-Lemma
-  exp_subst_ind (P : exp -> Prop) (Q : subst -> Prop)
-  : (forall n,  P (var n)) ->
-    (forall n s,  Q s -> P (con n s)) ->
-    Q [::] ->
-    (forall e s, P e -> Q s -> Q (e :: s)) ->
-    (forall e, P e) /\ (forall s, Q s).
-Proof using .
-  intros.
-  assert ( alleP : forall e, P e).
-  apply (@exp_subst_ind' P Q); auto.
-  split; auto.
-  clear H0 H.
-  suff: (forall e s, Q s -> Q (e :: s)).
-  intro; elim; eauto.
-  eauto.
-Qed.
-
-Lemma subst_cmp_size s1 s2 : size (subst_cmp s1 s2) = size s1.
-Proof using .
-  elim: s1; simpl; auto.
-Qed.
-
-Lemma exp_var_map_nth s' m s n
-  : exp_var_map (var_lookup s') (nth (var m) s n)
-    = nth (var_lookup s' m) (subst_cmp s s') n.
-Proof using .
-  elim: n s; intros until s; case: s => //=.
-Qed.
-
-Lemma var_lookup_cmp n s1 s2 : n < size s1 ->
-                               var_lookup (subst_cmp s1 s2) n = exp_var_map (var_lookup s2) (var_lookup s1 n).
-Proof using .
-  unfold var_lookup at 1 3; unfold nth_level.
-  rewrite !subst_cmp_size.
-  move => nlt; pose p := nlt; move: p.
-  case: (n < size s1) => //= _.
-  rewrite exp_var_map_nth.
-  move: nlt.
-  rewrite -!(@subst_cmp_size s1 s2) => nlt.
-  apply: set_nth_default.
-  move: nlt.
-  generalize (size (subst_cmp s1 s2)); case =>//.
-  intros; rewrite subSS.
-  apply: sub_ord_proof.
-Qed.
-
-Lemma subst_cmp_assoc'
-  : (forall e s1 s2, ws_exp (size s1) e -> e[/subst_cmp s1 s2/] = e[/s1/][/s2/])
-    /\ (forall s s1 s2, ws_subst (size s1) s -> subst_cmp (subst_cmp s s1) s2 = subst_cmp s (subst_cmp s1 s2)).
-Proof using .
-  apply exp_subst_ind; simpl; auto; intros.
-  2: by rewrite !con_subst_cmp H.
-  2: {
-    move /andP in H1.
-    destruct H1.
-    rewrite H; auto.
-    rewrite H0; auto.
-  }
- intros.
- unfold exp_subst.
- simpl.
- by apply var_lookup_cmp.
-Qed.
-
-Lemma subst_cmp_assoc s s1 s2
-  : List.fold_right (fun e : exp => andb (ws_exp (size s1) e)) true s ->
-    subst_cmp (subst_cmp s s1) s2 = subst_cmp s (subst_cmp s1 s2).
-Proof using .
-    by eapply subst_cmp_assoc'.
-Qed.
-
-Lemma sep_subst_cmp e s1 s2 :  ws_exp (size s1) e -> e[/subst_cmp s1 s2/] = e[/s1/][/s2/].
-Proof using .
-    by eapply subst_cmp_assoc'.
-Qed.
-
-(*TODO: needed?
-Fixpoint lift_subst sz n : subst :=
-  match sz with
-  | 0 => [::]
-  | sz'.+1 => (var n)::(lift_subst sz' (n.+1))
-  end.
-
-Lemma lift_subst_lookup n n0 sz : n < sz -> var (n0 + n) = var_lookup (lift_subst sz n0) n.
-Proof using .
-elim: n sz n0.
-    case; first easy; by simpl; intros; rewrite addn0.
-    move => n IH.
-    case; first easy.
-    intros; simpl.
-    rewrite -addSnnS.
-    eauto.
-Qed.
-
-Lemma lift_is_subst sz e n : ws_exp sz e -> e^!n = e[/lift_subst sz n/].
-Proof using .
-  case: e; unfold exp_subst; unfold exp_shift; simpl; eauto using lift_subst_lookup.
-  - intros.
-    f_equal.
-    apply: (map_ext' (P := ws_exp sz)); auto; intros.
-    apply: (exp_var_map_ext' (m:=sz)); auto; intros.
-    by apply: lift_subst_lookup.
-Qed. 
-
-
-Lemma subst_lift_is_subst sz s n : ws_subst sz s -> s^!!n = subst_cmp s (lift_subst sz n).
-Proof using .
-  elim: s n; simpl.
-  - elim: sz; simpl; auto.
-  - move => a l IH n /andP [wsa wsl].
-    f_equal; eauto using lift_is_subst.
-Qed.
-*)
-
-Fixpoint id_subst n : subst :=
-  match n with
-  | 0 => [::]
-  | n'.+1 =>
-    let s' := id_subst n' in
-    (var (size s'))::s'
-  end.
-
-Lemma id_subst_size sz : size (id_subst sz) = sz.
-Proof using .
-  elim: sz => //=.
-  intros; by f_equal.
-Qed.
-
-Lemma id_subst_lookup n sz : var_lookup (id_subst sz) n = var n.
-Proof using .
-  unfold var_lookup.
-  unfold nth_level.
-  rewrite id_subst_size.
-  case nsz: (n < sz) => //.
-  apply (level_ind (R:=fun m n => nth (var n) (id_subst sz) m = var n)); auto.
-  intro m.
-  elim: m n sz nsz; intros until sz; case: sz => //; simpl; intros.
-  - f_equal.
-    rewrite id_subst_size subn1.
-    by rewrite <-pred_Sn.
-  - rewrite !subSS.
-    eauto.
-Qed.    
-
-Lemma id_subst_identity e sz : e[/id_subst sz/] = e.
-Proof using .
-  elim: e sz; intros; unfold exp_subst; simpl; first by apply id_subst_lookup.
-  f_equal.
-  elim: l H => //.
-  simpl.
-  intro_to and.
-  case => [ aeq fld].
-  f_equal; eauto.    
-Qed.  
-
-Definition exp_of_uint ui := var (Nat.of_uint ui).
-Definition uint_of_exp e :=
-  match e with
-  | var n => Some (Nat.to_uint n)
-  | _ => None
-  end.
-
-Declare Scope exp_scope.
-Bind Scope exp_scope with exp.
-Delimit Scope exp_scope with exp_scope.
-Numeral Notation exp exp_of_uint uint_of_exp : exp_scope.
-
-Arguments con n s%exp_scope.
 *)
 
 (* TODO: how many of these should be part of the substable class?*)
