src/named/Tactics.v
@@ -158,8 +158,3 @@ Ltac2 inst_elab pat :=
   | _ => ()
   end.
 
-
-Ltac case_match :=match goal with
-  | [|- context[match ?e with _ => _ end]]
-    => let e':= fresh in remember e as e'; destruct e'
-  end.
